---

layout:     post
title:    "Note QS"
subtitle:   "CMPUT 204"
date:     2020-02-23
author:     "rick"
header-img: "img/post-c-language.png"
tags:
- Study note
---

##### The idea of quick sort

​	-- pick a pivot and compare it to all others

​	-- Rearrange A to be: [elements<= pivot, pivot, elements > pivot]

​	-- Recursively sort the subarrays of before and after elements

```
QuickSort(A,p,r)
		** sort the subarray A[p,...,r]
	if (p<r) then
		q <-- Partition(A,p,r)
			** Partition returns q such that
			** 1. A[q] is the pivot
			** 2. All elements <= pivot appear in A[p,...,q-1]
			** 3. All elements > pivot appear in A[q+1,...,r]
		QuickSort(A,p,q-1)
		QuickSort(A,q+1,r)
```

```
Partition(A,p,r)
	** last element, A[r], is the pivot key picked of the partition
	pivot <-- A[r]
	i <-- p-1
	for (j from p to r-1) do
		if (A[j] <= pivot) then
			i <-- i+1
			exchange A[i] <--> A[j]
	exchange A[i+1] <--> A[r]
	return i+1
```

##### Quick Sort running time

In each recurrence, there is n-1 Key comparisons because the pivot is compared with other n-1 keys.

​			0,                                   n<=1

T(n) =  			

​			T(n<sub>1</sub>)+T(n-1-n<sub>1</sub>)+(n-1), n>=2

n<sub>1</sub> + 1 is the index of the pivot. So quick sort needs 

T(All element before pivot)  + T(All element after pivot) + (n-1)

Notice that 0 <= n<sub>1</sub> <= n-1. Because the pivot can be any element from A[1] to A[n].

###### Worst case

When n1 is zero/n-1, the number of KC becomes T(0) + T(n-1) + (n-1). In the next level, the KC becomes n-2.

T(n) = T(n-1) + (n-1)

​		= T(n-1) + n-1 = T(n-2) + n-2 + n-1 = ... = T(1) + 1 + 2 + 3 + ... + n-1 = n(n-1)/2

So T(n) =  Θ(n^2)

###### Almost worst case

When n<sub>1</sub> is n-2 or 1, T(n) = T(1)+T(n-2)+(n-1)

​											= T(n-2)+(n-1) = T(n-4)+(n-3)+(n-1) = T(1) + 1 + 3 +...+ (n-1)

T(n) = (1+(n-1))n/4=n^2/4 = Θ(n^2)

###### Best case

If every time we can choose a pivot which makes # before and # after are same, then we can save all wasted KC.

T(n) = 2*T((n-1)/2)+(n-1)

Solving T(n) = 2T(n/2) + (n-1). Using master theorem second case, a = b =2, n^(log <sub>b</sub>a)=n. And f(n) = n-1 = n*((log^k)n) where k=0. So T(n) = (n*logn).

###### Almost best case

Assume in each round, # before is 3n/4 and # after is n/4. Then T(n) = T(3n/4)+T(n/4)+(n-1). Or more extreme case is T(n) = T(9n/10)+T(n/10)+(n-1).

In both case, the time is O(n*logn). For any split, the running time remains to be  Θ(nlogn).

